\documentclass{article}
\usepackage{parskip}
\usepackage{mathtools}
\usepackage{amsthm}

\begin{document}

\title{INF240 Mandatory Assignment 1}
\author{David Huynh}

\maketitle

\section*{Problem 1}

\subsection*{a)}
Fermat's theorem says that for $p$ prime and an integer $a$: $a^{p} \equiv a (mod p)$.\\
If $a$ does not divide $p$ then Fermat's theorem can be stated as: $a^{p-1} \equiv 1 (mod p)$-

To show that $n=55$ is composite we only need to test if $2^{n-1}
\equiv 1 (modn)$, this rule is given on p.80 in the textbook.\\
$2^{55-1} (mod$) $55 = 49 \neq 1$.\\
Thus $n=55$ is not prime and therefore composite

\subsection*{b)}

$n=341$ \hspace{5 mm} $k=3$\\
$n-1=340= 2^{2} \cdotp 85$ \hspace{5 mm} $s=2 \hspace{5mm} d=85$

\begin{tabular}{c | c | c | c | c | c}
Iteration & $a$ & $x$ & $x=1$ or $x=n-1?$ & $x_{2}$ & $x_{2}=1$ or $x_{2}=n-1?$\\ \hline

1 & 2 & $2^{85} (mod 341) = 32$ & no & $32^{2} (mod 341) = 1$ & yes\\
\end{tabular}

$n=341$ is composite since the algorithm stops for $a=2$

\subsection*{c)}

$x^{2} \equiv y^{2} (mod n)$ is a square congruence, from the principle on p.176 in the textbook $gcd(x-y,n)$ is a nontrivial factor of $n$.

Let us use a relation we obtained from b):\\
$32^{2} \equiv 1^{2} (mod$ $341)$\\
Find gcd with a version of Euclidian algorithm which states: 
\begin{verbatim}
procedure gcd(a,b) {
		if(a<b) swap(a,b)
		if(b ==0) return a
		return gcd(b, a mod b)
}
\end{verbatim}
This is equivalent to regular Euclidian algorithm per definition of modulus.
$
gcd(32-1, 341) = gcd(31, 341 \: mod \: 31) =  gcd(31,0). a = 31\\
gcd(32+1, 341) = gcd(33, 341 \: mod \: 33) =  gcd(33,11) = gcd(11, 33 \: mod \: 11) = gcd(11,0). a = 11\\
$
$341 = 11 \cdotp 31$

\section*{Problem 2}

\subsection*{a)}
$x^{2} \equiv c (mod \: p)$\\
We need to show that the equation only has a solution when $c^{(p-1)/2} = 1 (mod \: p)$.\\
Raise both sides to the power of $(p-1)/2$ and we obtain the following equation:\\
$x^{p-1} \equiv c^{(p-1)/2} (mod \: p)$, by Fermat's theorem $x^{p-1} \equiv 1 (mod \: p)$ so $c^{(p-1)/2}$ must equal $1 (mod \: p)$ or there are no solutions.

\subsection*{b)}

In the case where $p \equiv 3(mod \: 4)$ the solutions are given by the formula $x = \pm c^{(p+1)/4} (mod\:p)$ on lectures notes for chapter 3 slide 42.\\
$
x^{2} \equiv 5\:(mod \: 11)\\
x = \pm 5^{(11+1)/4}(mod \: 11)\\
x_{1} = 5^{3}(mod \: 11) = 4\\
x_{2} = -5^{3}(mod \: 11) = 7
$

$
x^{2} \equiv 12(mod \: 23)\\
x = \pm 12^{(23+1)/4}(mod \: 23)\\
x_{1} = 12^{6}(mod \: 23) = 9\\
x_{2} = -12^{6}(mod \: 23) = 14
$

\subsection*{c)}

Chinese remainder theorem (CRT) takes a sequence of coprime integers $m_{1}, m_{2} \ldots m_{r}$ and another set of integers $a_{1}, a_{2} \ldots a_{r}$\\
It then creates a system of $r$ linear congruences of the form $x \equiv a_{i} (mod \: m_{i})$ and finds a unique solution $x \: mod \: (m_{1}m_{2}\ldots m_{r}$

We want to solve $x^{2} \equiv 104 (mod \: 253)$\\
Notice that $253 = 11 \cdotp 23$ so we can set up the system:

$x^{2} \equiv 104 (mod \: 11)$\\
$x^{2} \equiv 104 (mod \: 23)$\\
Solutions follow from same principle as in 2b)

$x \equiv \pm 104^{(11+1)/4} (mod \: 11)$
$x \equiv \pm 104^{3} (mod \: 11) = \pm 4 (mod \: 11)$

$x \equiv \pm 104^{(23+1)/4} (mod \: 23)$
$x \equiv \pm 104^{6} (mod \: 23) = \pm 9 (mod \: 23)$

Now combine the solutions using CRT, I use the algorithm described on p.108, exercise 24 in the textbook. I made the program EEA.cpp to find modular inverse:\\
$M = m_{1} \cdotp m_{2} = 11 \cdotp 23 = 253$\\
$z_{1} = 23$\\
$y_{1} \equiv  23^{-1} (mod \: 11) = 1$

$z_{2} = 11$\\
$y_{2} \equiv 11^{-1} (mod \: 23) = -2 \: mod \: 23 = 21$

$x$ has solutions on the form $x_{i} = a_{1} \cdotp 23 \cdotp 1 + a_{2} \cdotp 11 \cdotp 21$ where $a_{1} = \pm 4 (mod \: 11)$ and $a_{2} = \pm 9 (mod \: 23)$.

$x_{1} = 4 \cdotp 23 + 9 \cdotp 11 \cdotp 21 (mod \: 253) = 2171 (mod \: 253) = 147$\\
$x_{2} = 4 \cdotp 23 - 9 \cdotp 11 \cdotp 21 (mod \: 253) = -1987 (mod \: 253) = 37$\\
$x_{3} = -4 \cdotp 23 + 9 \cdotp 11 \cdotp 21 (mod \: 253) = 1987 (mod \: 253) = 216$\\
$x_{4} = -4 \cdotp 23 - 9 \cdotp 11 \cdotp 21 (mod \: 253) = -2171 (mod \: 253) = 106$\\

\subsection*{d)}
By statement in a) we must choose $c$ such that $c^{(p-1)/2} \neq 1(mod \: p)$, so:\\
$c^{(253-1)/2} \neq 1 (mod \: 253)$
$c^{126} \neq 1 (mod \: 253)$

One solution is $c=2$, quick check shows $2^{126} mod \: 253 = 9 \neq 1$.

\section*{Problem 3}

$p = 19, \hspace{5 mm} q = 23\\
n = pq = 437 \hspace{5 mm} \phi(n) = (p-1)(q-1) = 396$

\subsection*{a)}
$e = 7$\\
I made the program EEA.cpp with $a=7$ and $b=396$ to compute private exponent $d=283$

RSA encryption is done by $c \equiv m^{e}(mod \: n)$, so with $m=5$ encryption is as follows:\\
$c(5) = 5^{7}(mod \: 437) = 339$

\subsection*{b)}

We need to choose an $e_{A}$ such that $1 < e_{A} < \phi(n)$ and $gcd(e_{A}, \phi(n)) = 1$, $e_{A} = 5$ satisfies these conditions. Our $d_{A}$ is then $d_{A} \equiv e_{A}^{-1} (mod \: \phi(n))$, again I use the program EEA.cpp with $a=e_{A}=5$ and $b=\phi(n)=396$ to compute $d_{A}=317$.

By description on p.245 in the textbook, signing is done by the formula $y \equiv m^{d_{A}} (mod \: n)$, plugging in for $m=2$ gives us:\\
$y \equiv 2^{317} (mod \: 437) = 167$.

Verification is also described on p.245 and is given by testing if $z \equiv y^{e_{A}} (mod \: n) = m$, where $e_{A}$ and $n$ are respectively the sender's public key and product of $pq$.\\
$z \equiv 167^{5} (mod \: 437) = 2$

\section*{Problem 4}

$3^{x} = 5(mod \: 29)$

\subsection*{a)}
Using the Pohlig-Hellman algorithm:

$29-1 = 2^{2} \cdotp 7 \hspace{5mm} \alpha = 3 \hspace{5mm} \beta = 5$

$5 (mod \: 2^{2})$ and $5 (mod \: 7$

$q=2, \hspace{5mm} r=2$ so we must now find $x mod \: 2^{2}$\\
$x \equiv x_{0} + 2x_{1} (mod \: 4)$\\
$\beta^{(p-1)/q} = 5^{14} = 1 (mod \: 29)$\\
$(3^{14})^{x_{0}} = 28^{x_{0}} (mod \: 29)$\\
We must find $x_{0}$ such that the alpha and beta expressions are equivalent.
Try $x_{0} = 0$ gives $1 (mod \: 29)$ so $x_{0} = 0$

Now we must find $x_{1}$\\
$\beta_{1} \equiv \beta \alpha^{-x_{0}} \equiv 5 \cdotp 3^{-0} \equiv 5$\\
$\beta_{1}^{(p-1)/2^{2}} \equiv 5^{7} \equiv 28 (mod \: 29)$\\
$(\alpha^{(p-1)/q})^{x_{1}} \equiv 28^{x_{1}} (mod \: 29) \Rightarrow x_{1} = 1$

$x \equiv x_{0} + 2x_{1} \equiv 0 + 2 \equiv 2 (mod \: 4)$

Next to solve $x mod \: 7$\\
$q=7, \hspace{5mm} r=1$\\
$x \equiv x_{0} (mod \: 7)$\\
$\beta^{(p-1)/q} \equiv 5^{4} \equiv 16 (mod \: 29)$\\
$\alpha^{(p-1)/q} \equiv 3^{4} \equiv 23 (mod \: 29)$\\

Trying all possible values of $x_{0}$ we get:\\
$23^{2} \equiv 7, \hspace{5mm} 23^{3} \equiv 16 (mod \: 29) \Rightarrow x_{0} = 3$\\
$x \equiv 3 (mod \: 7)$

Using CRT to combine $x \equiv 2 (mod \: 4)$ and $x \equiv 3 (mod \: 7$ gives us $x \equiv 10 (mod \: 29)$

\subsection*{b)}

Using the index-calculus method:\\
$p=29, \hspace{5mm} \alpha=3, \hspace{5mm} B=\{2,3,5,7\}$

Precomputation:\\
$
3^{1} \equiv 3 (mod \: 29)\\
3^{2} \equiv 3^{2} (mod \: 29)\\
3^{3} \equiv 3^{3} (mod \: 29\\
3^{6} \equiv 2^{2} (mod \: 29)\\
3^{7} \equiv 2^{2} \cdotp 3 (mod \: 29)
$

We get:\\
$
1 \equiv L_{3}(3) (mod \: 28)\\
2 \equiv 2L_{3}(3) (mod \: 28)\\
3 \equiv 3L_{3}(3) (mod \: 28)\\
6 \equiv 2L_{3}(2) (mod \: 28)\\
7 \equiv 2L_{3}(2) + L_{3}(3) (mod \: 28)
$

\subsection*{c)}
$p = 29, \hspace{5mm} \alpha=3$, $\alpha$ being a primitive root can be shown by successively computing $\alpha^{i} (mod \: p)$ and increasing $i$ by 1 several times and it will generate the complete order mod p, that is, all numbers from 0 to p-1 mod p.

Choosing random $x=5, \hspace{5mm} y=7$\\
Next we compute $\alpha^{x} (mod \: p)$ and $\alpha^{y} (mod \: p)$:\\
$3^{5} (mod \: 29) = 11, \hspace{5mm} 3^{7} (mod \: 29) = 12$\\

Lastly we compute they key $K$ by $K \equiv (\alpha^{y})^{x} (mod \: p)$ and $K \equiv (\alpha^{x})^{y} (mod \: p)$:\\
$(3^{7})^{5} (mod \: 29) = 12$\\
$(3^{5})^{7} (mod \: 29) = 12$

\end{document}
